progress towards new examply with monotone calling convention

theories/examples/stack_object.v
@@ -1,7 +1,7 @@
 From iris.algebra Require Import frac.
 From iris.proofmode Require Import tactics.
 Require Import Eqdep_dec List.
-From cap_machine Require Import rules logrel fundamental region_invariants_revocation region_invariants_static region_invariants_batch_uninitialized.
+From cap_machine Require Import rules rules_LoadU_derived logrel fundamental region_invariants_revocation region_invariants_static region_invariants_batch_uninitialized stack_object_helpers.
 From cap_machine Require Export iris_extra addr_reg_sample region_macros contiguous stack_macros_helpers macros.
 
 Section stack_object.
@@ -19,34 +19,367 @@ Section stack_object.
   Definition r_param1 := r_t16.
   Definition r_param2 := r_t17.
 
-  Definition stack_object_passing_instrs stack_obj :=
+  Definition stack_object_passing_instrs stack_obj f_a :=
     (* we check that the function pointer is global *)
     reqglob_instrs r_adv ++
-    (* we must do some dynamic checks on the input object *)
+    (* prepare the stack *)
+    prepstackU_instrs r_stk 12 2 ++
+    (* load parameter 1 into register *)
+    [loadU_r_z r_param1 r_stk (-1)] ++
+    (* we must do some dynamic checks on the input object, which can be a stack object *)
     checkra_instrs r_param1 ++
     checkints_instrs r_param1 r_t1 r_t2 r_t3 ++
-    (* prepare the stack *)
-    prepstackU_instrs r_stk 9 ++
-    checkbelow_instrs r_t0 r_stk ++
     (* we can begin the function *)
-    [pushU_z_instr r_stk stack_obj;
+    (* push some local state *)
+    [pushU_z_instr r_stk 2;
+    (* we create a stack object *)
+    pushU_z_instr r_stk stack_obj;
     move_r r_param2 r_stk;
-    promoteU r_param2;
-    (* push the local state *)
-    pushU_r_instr r_stk r_t0] ++
+    getb r_t1 r_stk;
+    gete r_t2 r_stk;
+    add_r_z r_t1 r_t1 3;
+    subseg_r_r r_param2 r_t1 r_t2;
+    promoteU r_param2] ++
     (* call r_adv *)
     scallU_prologue_instrs r_adv [r_param1;r_param2] ++
-    [ jmp r_adv;
+    (* we push the parameters onto the new restricted adversary stack *)
+    [pushU_r_instr r_stk r_param1;
+    pushU_r_instr r_stk r_param2;
+    pushU_r_instr r_stk r_t0;
+    move_z r_param1 0; (* these three cleanup steps are not necessary, but practical *)
+    move_z r_param2 0;
+    move_z r_t0 0;
+    (* jump to the ardversary callee *)
+    jmp r_adv;
     (* restore local state *)
     lea_z r_stk (-6)] ++
-    popU_instrs r_stk r_t0 ++
-    (* we leave everything on the stack *)
+    (* we assert that the local state is still 2. If the return pointer has been leaked,
+       then the caller can alter the local state, jump to the return pointer and make
+       the following assertion fail *)
+    [loadU_r_z r_t1 r_stk (-2)] ++
+    assert_r_z_instrs f_a r_t1 2 ++
+    [loadU_r_z r_t0 r_stk (-4)] ++
+    (* we leave everything on the stack, but clear registers before returning *)
     rclear_instrs (list_difference all_registers [PC;r_t0]) ++
     [jmp r_t0].
 
-  Definition stack_object_passing a p f_a :=
-    ([∗ list] a_i;w_i ∈ a;(stack_object_passing_instrs f_a), a_i ↦ₐ[p] w_i)%I.
-  
+  Definition stack_object_passing a p stack_obj f_a :=
+    ([∗ list] a_i;w_i ∈ a;(stack_object_passing_instrs stack_obj f_a), a_i ↦ₐ[p] w_i)%I.
+
+
+  Lemma stack_object_spec W pc_p pc_p' pc_g pc_b pc_e (* PC *)
+        stack_object_passing_addrs (* program addresses *)
+        a_first a_last (* special adresses *)
+        f_a b_link e_link a_link a_entry fail_cap (* linking table variables *)
+        stack_obj advw (* input *)
+        wstk (* stack *)
+        rmap (* registers *)
+        ι1 ι2 (* invariant names *) :
+
+    (* PC assumptions *)
+    isCorrectPC_range pc_p pc_g pc_b pc_e a_first a_last ->
+    PermFlows pc_p pc_p' ->
+
+    (* Program adresses assumptions *)
+    contiguous_between stack_object_passing_addrs a_first a_last ->
+
+    (* Linking table assumptions *)
+    withinBounds (RW, Global, b_link, e_link, a_entry) = true →
+    (a_link + f_a)%a = Some a_entry ->
+
+    (* the monotonicity of the PC is not monotone *)
+    isMonotone pc_g = false →
+
+    (* footprint of the register map *)
+    dom (gset RegName) rmap = all_registers_s ∖ {[PC;r_stk;r_adv]} →
+
+    (* The two invariants have different names *)
+    (up_close (B:=coPset) ι2 ## ↑ι1) ->
+
+    {{{ r_stk ↦ᵣ wstk
+      ∗ PC ↦ᵣ inr ((pc_p,pc_g),pc_b,pc_e,a_first)
+      ∗ ([∗ map] r_i↦w_i ∈ rmap, r_i ↦ᵣ w_i)
+      (* adv *)
+      ∗ r_adv ↦ᵣ advw
+      ∗ interp W advw
+      (* stack *)
+      ∗ interp W wstk
+      (* token which states all non atomic invariants are closed *)
+      ∗ na_own logrel_nais ⊤
+      (* trusted code *)
+      ∗ na_inv logrel_nais ι1 (stack_object_passing stack_object_passing_addrs pc_p' stack_obj f_a)
+      (* linking table *)
+      ∗ na_inv logrel_nais ι2 (pc_b ↦ₐ[pc_p'] inr (RO,Global,b_link,e_link,a_link) ∗ a_entry ↦ₐ[RO] fail_cap)
+      (* we start out with arbitrary sts *)
+      ∗ sts_full_world W
+      ∗ region W
+    }}}
+      Seq (Instr Executable)
+      {{{ v, RET v; ⌜v = HaltedV⌝ →
+                    ∃ r W', full_map r ∧ registers_mapsto r
+                         ∗ ⌜related_sts_priv_world W W'⌝
+                         ∗ na_own logrel_nais ⊤
+                         ∗ sts_full_world W'
+                         ∗ region W' }}}.
+  Proof.
+    iIntros (Hvpc Hfl Hcont Hlt_wb Hlt_link Hpcmono Hdom Hndisj φ).
+    iIntros "(Hr_stk & HPC & Hregs & Hr_adv & #Hadv_valid & #Hwstk_valid & Hown & #Hlse_prog & #Htable & Hsts & Hr) Hφ".
+    iMod (na_inv_acc with "Hlse_prog Hown") as "(>Hprog & Hown & Hcls)";auto.
+
+    (* get some general purpose registers *)
+    assert (is_Some (rmap !! r_t0)) as [w0 Hw0];[apply elem_of_gmap_dom;rewrite Hdom;set_solver+|].
+    assert (is_Some (rmap !! r_t1)) as [w1 Hw1];[apply elem_of_gmap_dom;rewrite Hdom;set_solver+|].
+    assert (is_Some (rmap !! r_t2)) as [w2 Hw2];[apply elem_of_gmap_dom;rewrite Hdom;set_solver+|].
+    assert (is_Some (rmap !! r_t3)) as [w3 Hw3];[apply elem_of_gmap_dom;rewrite Hdom;set_solver+|].
+    assert (is_Some (rmap !! r_t4)) as [w4 Hw4];[apply elem_of_gmap_dom;rewrite Hdom;set_solver+|].
+    assert (is_Some (rmap !! r_param1)) as [wp1 Hwp1];[apply elem_of_gmap_dom;rewrite Hdom;set_solver+|].
+    assert (is_Some (rmap !! r_param2)) as [wp2 Hwp2];[apply elem_of_gmap_dom;rewrite Hdom;set_solver+|].
+    iDestruct (big_sepM_delete with "Hregs") as "[Hr_t0 Hregs]";[apply Hw0|].
+    iDestruct (big_sepM_delete _ _ r_t1 with "Hregs") as "[Hr_t1 Hregs]";[rewrite lookup_delete_ne//;eauto|].
+    iDestruct (big_sepM_delete _ _ r_t2 with "Hregs") as "[Hr_t2 Hregs]";[rewrite !lookup_delete_ne//;eauto|].
+    iDestruct (big_sepM_delete _ _ r_t3 with "Hregs") as "[Hr_t3 Hregs]";[rewrite !lookup_delete_ne//;eauto|].
+    iDestruct (big_sepM_delete _ _ r_t4 with "Hregs") as "[Hr_t4 Hregs]";[rewrite !lookup_delete_ne//;eauto|].
+    iDestruct (big_sepM_delete _ _ r_param1 with "Hregs") as "[Hr_param1 Hregs]";[rewrite !lookup_delete_ne//;eauto|].
+    iDestruct (big_sepM_delete _ _ r_param2 with "Hregs") as "[Hr_param2 Hregs]";[rewrite !lookup_delete_ne//;eauto|].
+
+    (* reqglob  *)
+    iPrologue_multi "Hprog" Hcont Hvpc link.
+    iApply (reqglob_spec with "[- $HPC $Hcode $Hr_adv]");[eauto..|].
+    iSplitL "Hr_t1";[eauto|]. iSplitL "Hr_t2";[eauto|].
+    iNext. destruct (isGlobalWord advw) eqn:Hglob;[|(* Failure *) iApply "Hφ";iIntros (Hcontr);inversion Hcontr].
+    destruct advw as [c | [ [ [ [g l] b] e] a'] ];[inversion Hglob|]. destruct l;[|inversion Hglob..].
+    iExists _,_,_,_. iSplit;[eauto|].
+    iIntros "(HPC & Hreqglob & Hr_adv & Hr_t1 & Hr_t2)".
+
+    (* prepstack *)
+    iPrologue_multi "Hprog" Hcont Hvpc link0.
+    iApply (prepstackU_spec with "[- $HPC $Hcode $Hr_stk]");[eauto..|].
+    iSplitL "Hr_t1";[eauto|]. iSplitL "Hr_t2";[eauto|].
+    iNext. destruct (isPermWord wstk URWLX) eqn:Hperm;[|(* Failure *) iApply "Hφ";iIntros (Hcontr);inversion Hcontr].
+    destruct wstk as [c | [ [ [ [gstk lstk] bstk] estk] astk] ];[inversion Hperm|]. destruct gstk;inversion Hperm.
+    iExists _,_,_,_. iSplit;[eauto|].
+    destruct ((12%nat + 2%nat <? estk - bstk)%Z) eqn:Hsize;[|(* Failure *) iApply "Hφ";iIntros (Hcontr);inversion Hcontr].
+    destruct ((bstk + 2%nat <=? astk)%Z) eqn:Hbounds;[|(* Failure *) iApply "Hφ";iIntros (Hcontr);inversion Hcontr].
+    iIntros "Hcont". iDestruct "Hcont" as (a_param Ha_param) "(HPC & HprepstackU & Hr_stk & Hr_t1 & Hr_t2)".
+    apply Z.ltb_lt in Hsize. apply Z.leb_le in Hbounds.
+
+    (* we can extract the validity of the parameters passed on the stack *)
+    iDestruct (read_allowedU_inv _ bstk with "Hwstk_valid") as (p' Hflows) "Hcond1";[clear -Hbounds Hsize Ha_param;solve_addr|auto|].
+    iDestruct (writeLocalAllowedU_valid_cap_below_implies _ _ _ _ _ _ bstk with "Hwstk_valid") as %Hmono1;
+      [auto|apply le_addr_withinBounds|..];[clear -Hbounds Hsize Ha_param;solve_addr..|].
+    destruct p';inversion Hflows;clear Hflows.
+
+    destruct (bstk + 1)%a eqn:Hsome;[|exfalso;clear -Ha_param Hsome;solve_addr].
+    iDestruct (read_allowedU_inv _ a with "Hwstk_valid") as (p' Hflows) "Hcond2";[clear -Hbounds Hsize Hsome;solve_addr|auto|].
+    iDestruct (writeLocalAllowedU_valid_cap_below_implies _ _ _ _ _ _ a with "Hwstk_valid") as %Hmono2;
+      [auto|apply le_addr_withinBounds|..];[clear -Hbounds Hsize Hsome;solve_addr..|].
+    destruct p';inversion Hflows;clear Hflows.
+
+    (* loadU r_param1 r_stk -1 *)
+    iPrologue_multi "Hprog" Hcont Hvpc link1.
+    iDestruct (big_sepL2_length with "Hcode") as %Hprog_length.
+    destruct_addr_list l_code1.
+    iDestruct (region_open_monotemp_pwl with "[$Hcond2 $Hr $Hsts]") as
+        (wsecret) "(Hr & Hsts & Hstate & Ha & % & #Hmono & #Hwsecret_valid)";[auto..|].
+    iPrologue "Hcode". apply contiguous_between_cons_inv_first in Hcont_code1 as Heq. subst l_code1.
+    iApply (wp_loadU_success with "[$HPC $Hi $Hr_param1 $Hr_stk $Ha]");
+      [apply decode_encode_instrW_inv|apply Hfl|auto|iCorrectPC link0 link1|auto..].
+    { clear -Hsome Ha_param Hbounds Hsize. apply le_addr_withinBounds;solve_addr. }
+    { apply Hlink1. }
+    { clear -Hsome Ha_param Hbounds Hsize. solve_addr. }
+    iEpilogue "(HPC & Hr_param1 & Hprog_done & Hr_stk & Ha)".
+    iDestruct (region_close_monotemp_pwl with "[$Hstate $Hr $Ha $Hcond2]") as "Hr";auto. iClear "Hcode".
+
+    (* check the passed object is RA *)
+    iPrologue_multi "Hprog" Hcont Hvpc link2.
+    iApply (checkra_spec with "[- $HPC $Hcode $Hr_param1 $Hr_t1 $Hr_t2 $Hr_t3 $Hr_t4]");[eauto..|].
+    iNext. destruct (is_cap wsecret) eqn:Hiscap;[|(* Failure *) iApply "Hφ";iIntros (Hcontr);inversion Hcontr].
+    destruct wsecret as [c | [ [ [ [l p] bsec] esec] asec] ];[inversion Hiscap|].
+    iExists _,_,_,_,_;iSplit;[eauto|].
+    destruct (readAllowed l) eqn:Hra;[|(* Failure *) iApply "Hφ";iIntros (Hcontr);inversion Hcontr].
+    iIntros "(HPC & Hcheckra & Hr_param1 & Hr_t1 & Hr_t2 & Hr_t3 & Hr_t4)".
+
+    (* we must now dynamically check that the object in param1 is of the correct type *)
+    (* we must therefore extract the object from W *)
+    (* we will thereafter need to freeze the full world, before reinstating the object after the check *)
+
+    (* extract region information of [bsec,esec] from W *)
+    iDestruct (state_unused_stack with "Hwstk_valid") as %Hstack_state;[apply Hbounds|apply Ha_param|].
+    iDestruct (input_stack_disjoint _ _ a_param estk with "[$Hwsecret_valid $Hmono]") as %Hdisj;
+      [clear -Hbounds Hsize Hsome Ha_param;solve_addr|auto|auto|].
+    iDestruct (readAllowed_implies_region_conditions with "Hwsecret_valid") as "Hsecret_cond";auto.
+
+    (* uninitialize the full stack *)
+    iMod (uninitialize_region_keep _ addr_reg.za with "[$Hsts $Hr]") as (m Hmcond) "[Hsts [Hr #Hvalids] ]".
+    (* next we can open the region at b_stk, which we will first assert is in m *)
+    iDestruct (valid_uninitialized_condition_weak _ m with "Hwstk_valid") as %Hstk_cond;eauto. clear. solve_addr.
+    iSimpl in "Hwsecret_valid". iDestruct (valid_readAllowed_condition_weak _ m with "Hwsecret_valid") as %Hsec_cond;eauto. clear. solve_addr.
+
+    (* opening [bsec,esec] while remembering the words in case of uninitialized state in (uninit m W) *)
+    iDestruct (open_stack_object with "[$Hsts $Hr]") as "(Hsts & Hws)";eauto.
+    { iApply big_sepL_forall. iIntros (k x Hx).
+      assert (x ∈ region_addrs bsec esec) as Hinx;[apply elem_of_list_lookup;eauto|].
+      iApply read_allowed_inv. apply elem_of_region_addrs in Hinx. eauto. eauto.
+      iFrame "Hwsecret_valid". }
+    iDestruct "Hws" as (wps) "(Hbesec & Hcls' & #Hsecret_states & #Hperms)".
+    iDestruct "Hsecret_states" as %Hsecret_states. iDestruct "Hperms" as %Hperm_flows.
+
+    (* Now we are ready to apply the checkints macro *)
+    iPrologue_multi "Hprog" Hcont Hvpc link3.
+    iApply (wp_wand with "[- Hφ]").
+    2: { iIntros (v) "Hφ'". iApply "Hφ". iExact "Hφ'". }
+    iApply (wp_wand with "[-]").
+    iApply (checkints_spec with "[- $HPC $Hcode $Hr_param1 $Hbesec $Hr_t1 $Hr_t2 $Hr_t3]");[eauto..|].
+    2: { iSimpl. iIntros (v) "[Hφ | Hfailed]". iExact "Hφ". iIntros "Hcontr". iSimplifyEq. }
+    iNext. iIntros "(HPC & Hcheckints & Hr_param1 & Hr_t1 & Hr_t2 & Hr_t3 & Hbesec & #Hints)".
+    iDestruct "Hints" as %Hints.
+    (* we now have enough information to close the region again *)
+    iDestruct ("Hcls'" with "Hbesec") as "Hr".
+
+    (* for the next part of the code, we will need to manipulate our local stack frame *)
+    (* for that, we begin by revoking the full local stack frame from W *)
+    assert (∃ frame_end, a_param + 10 = Some frame_end)%a as [frame_end Hframe_delim].
+    { clear -Hbounds Ha_param Hsome Hsize. destruct (a_param + 10)%a eqn:HH;eauto. exfalso. solve_addr.}
+    (* first we must know that a fully uninitialized world satisfies the revoke condition *)
+    apply uninitialize_revoke_condition in Hmcond as Hrevoked.
+    (* next we may revoke it *)
+    iMod (uninitialize_to_revoked_cond_states (region_addrs bstk frame_end) _ _ RWLX (λ Wv, interp Wv.1 Wv.2) with "[$Hr $Hsts]") as "(Hr & Hsts & Hframe)";[apply region_addrs_NoDup|auto|..].
+    { apply Forall_forall. intros x Hin%elem_of_region_addrs. apply Hstk_cond. clear -Hbounds Ha_param Hsome Hsize Hframe_delim Hin. solve_addr. }
+    { iApply big_sepL_forall. iIntros (k x Hlookup).
+      assert (x ∈ (region_addrs bstk frame_end)) as Hin;[apply elem_of_list_lookup;eauto|].
+      apply elem_of_region_addrs in Hin.
+      iDestruct (read_allowedU_inv _ x with "Hwstk_valid") as (p' Hflows) "Hcond".
+      clear -Hin Hframe_delim Ha_param Hsome Hsize Hbounds. solve_addr.
+      auto. destruct p';inversion Hflows. iFrame "Hcond". }
+
+    (* finally we clean up our resources a bit *)
+    iAssert (∃ ws wret w', bstk ↦ₐ[RWLX] wret ∗ a ↦ₐ[RWLX] w' ∗ [[a_param,frame_end]]↦ₐ[RWLX][[ws]])%I with "[Hframe]" as (wsstk wret w') "(Hbstk & Ha & Hframe)".
+    { iDestruct (region_addrs_exists with "Hframe") as (ws) "Hframe".
+      iDestruct (big_sepL2_length with "Hframe") as %Hflen. rewrite region_addrs_length in Hflen.
+      assert (region_size bstk frame_end = 12) as Heq. clear -Hframe_delim Ha_param. rewrite /region_size. solve_addr.
+      rewrite Heq in Hflen. destruct ws;[inversion Hflen|]. rewrite region_addrs_cons;[|clear -Hframe_delim Ha_param;solve_addr].
+      rewrite Hsome /=. rewrite region_addrs_cons;[|clear -Hframe_delim Ha_param Hsome;solve_addr].
+      assert ((a + 1)%a = Some a_param) as ->;[clear -Hsome Ha_param;solve_addr|]. destruct ws;[inversion Hflen|]. simpl.
+      iDestruct "Hframe" as "(H1 & H2 & Hframe)".
+      iExists ws,w,w5. iDestruct "H1" as "[_ $]". iDestruct "H2" as "[_ $]".
+      iApply (big_sepL2_mono with "Hframe"). iIntros (k y1 y2 Hin1 Hin2) "[_ H]". iFrame. }
+    iDestruct (big_sepL2_length with "Hframe") as %Hframe_length.
+    rewrite region_addrs_length in Hframe_length.
+    apply (incr_addr_region_size_iff _ _ 10)in Hframe_delim as Hframe_det.
+    destruct Hframe_det as [Hframe_le Hframe_size]. rewrite Hframe_size in Hframe_length.
+
+    (* we can now continue with the execution of instructions *)
+    iPrologue_multi "Hprog" Hcont Hvpc link4.
+    iDestruct (big_sepL2_length with "Hcode") as %Hlength_code.
+    destruct_addr_list l_code3.
+    iDestruct (writeLocalAllowedU_implies_local with "Hwstk_valid") as %Hmono;auto.
+    destruct lstk;inversion Hmono;clear Hmono.
+
+    (* pushU r_stk 2 *)
+    assert (is_Some (a_param + 1)%a) as [af2 Haf2].
+    { destruct (a_param + 1)%a eqn:Hcontr;eauto;exfalso;clear -Hframe_delim Hcontr;solve_addr. }
+    destruct wsstk as [|wf1 wsstk];[inversion Hframe_length|].
+    iDestruct (region_mapsto_cons with "Hframe") as "[Hf1 Hframe]";
+      [apply Haf2|clear -Haf2 Hframe_delim;solve_addr|..].
+    iDestruct "Hcode" as "[Hi Hcode]".
+    apply contiguous_between_cons_inv_first in Hcont_code4 as Heq. subst l_code3.
+    iApply (pushU_z_spec with "[- $HPC $Hf1 $Hr_stk $Hi]");
+      [iCorrectPC link3 link4|apply Hfl|auto| |iContiguous_next_a Hcont_code4|apply Haf2|].
+    { clear -Hbounds Ha_param Hsize Hframe_delim. apply le_addr_withinBounds; solve_addr. }
+    iNext. iIntros "(HPC & Hprog_done2 & Hr_stk & Hf1)".
+
+    (* pushU r_stk stack_obj *)
+    assert (is_Some (af2 + 1)%a) as [af3 Haf3].
+    { destruct (af2 + 1)%a eqn:Hcontr;eauto;exfalso;clear -Hframe_delim Hcontr Haf2;solve_addr. }
+    destruct wsstk as [|wf2 wsstk];[inversion Hframe_length|].
+    iDestruct (region_mapsto_cons with "Hframe") as "[Hf2 Hframe]";
+      [apply Haf3|clear -Haf2 Haf3 Hframe_delim;solve_addr|..].
+    iDestruct "Hcode" as "[Hi Hcode]".
+    iApply (pushU_z_spec with "[- $HPC $Hf2 $Hr_stk $Hi]");
+      [iCorrectPC link3 link4|apply Hfl|auto| |iContiguous_next_a Hcont_code4|apply Haf3|].
+    { clear -Hbounds Ha_param Hsize Hframe_delim Haf2 Haf3.
+      apply le_addr_withinBounds; solve_addr. }
+    iNext. iIntros "(HPC & Hi & Hr_stk & Hf2)". iCombine "Hi" "Hprog_done2" as "Hprog_done2".
+
+    (* move r_param2 r_stk *)
+    iPrologue "Hcode".
+    iApply (wp_move_success_reg with "[$HPC $Hi $Hr_param2 $Hr_stk]");
+      [apply decode_encode_instrW_inv|apply Hfl|iCorrectPC link3 link4|iContiguous_next_a Hcont_code4|].
+    iEpilogue "(HPC & Hi & Hr_param2 & Hr_stk)"; iCombine "Hi" "Hprog_done2" as "Hprog_done2".
+    (* getb r_t1 r_stk *)
+    iPrologue "Hcode".
+    iApply (wp_Get_success with "[$HPC $Hi $Hr_t1 $Hr_stk]");
+      [apply decode_encode_instrW_inv|eauto|apply Hfl|iCorrectPC link3 link4|iContiguous_next_a Hcont_code4|auto..|].
+    iEpilogue "(HPC & Hi & Hr_stk & Hr_t1)"; iCombine "Hi" "Hprog_done2" as "Hprog_done2".
+    iSimpl in "Hr_t1".
+    (* gete r_t2 r_stk *)
+    iPrologue "Hcode".
+    iApply (wp_Get_success with "[$HPC $Hi $Hr_t2 $Hr_stk]");
+      [apply decode_encode_instrW_inv|eauto|apply Hfl|iCorrectPC link3 link4|iContiguous_next_a Hcont_code4|auto..|].
+    iEpilogue "(HPC & Hi & Hr_stk & Hr_t2)"; iCombine "Hi" "Hprog_done2" as "Hprog_done2".
+    iSimpl in "Hr_t2".
+    (* add r_t1 r_t1 3 *)
+    iPrologue "Hcode".
+    iApply (wp_add_sub_lt_success_dst_z with "[$HPC $Hi $Hr_t1]");
+      [apply decode_encode_instrW_inv|eauto|iContiguous_next_a Hcont_code4|apply Hfl|iCorrectPC link3 link4|].
+    iEpilogue "(HPC & Hi & Hr_t1)"; iCombine "Hi" "Hprog_done2" as "Hprog_done2".
+    iSimpl in "Hr_t1".
+    (* subseg r_param2 r_t1 r_t2 *)
+    iPrologue "Hcode".
+    iApply (wp_subseg_success _ _ _ _ _ _ _ _ _ _ _ _ _ _ _ _ _ af2 estk with "[$HPC $Hi $Hr_param2 $Hr_t1 $Hr_t2]");
+      [apply decode_encode_instrW_inv|apply Hfl|iCorrectPC link3 link4| |auto|auto| |iContiguous_next_a Hcont_code4|].
+    { split;[|apply z_to_addr_z_of]. clear -Haf2 Ha_param. assert (bstk + 3 = Some af2)%a;[solve_addr|].
+      apply incr_addr_of_z_i in H as Heq. rewrite Heq. apply z_to_addr_z_of. }
+    { rewrite /isWithin. apply andb_true_iff. rewrite !Z.leb_le. clear -Ha_param Haf2. solve_addr. }
+    iEpilogue "(HPC & Hi & Hr_t1 & Hr_t2 & Hr_param2)"; iCombine "Hi" "Hprog_done2" as "Hprog_done2".
+    (* promoteU r_param2 *)
+    iPrologue "Hcode".
+    iApply (rules_PromoteU_derived.wp_promoteU_success with "[$HPC $Hi $Hr_param2]");
+      [apply decode_encode_instrW_inv|apply Hfl|iCorrectPC link3 link4|auto|..].
+    { eapply contiguous_between_last. apply Hcont_code4. auto. }
+    iEpilogue "(HPC & Hi & Hr_param2)"; iCombine "Hi" "Hprog_done2" as "Hprog_done2".
+    iSimpl in "Hr_param2". assert (addr_reg.min af3 estk = af3) as ->;[clear -Hbounds Hsize Ha_param Haf2 Haf3;solve_addr|].
+
+    (* we are now ready to apply the calling convention *)
+    (* split up the stack frame into activation and parameter part *)
+    assert (∃ a_r_adv, (af3 + 6)%a = Some a_r_adv) as [a_r_adv Ha_r_adv];
+      [clear -Hbounds Hframe_delim Haf2 Haf3;destruct (af3 + 6)%a eqn:hsome;eauto;exfalso;solve_addr|].
+    assert (∃ b_r_adv, (af3 + 7)%a = Some b_r_adv) as [b_r_adv Hb_r_adv];
+      [clear -Hbounds Hframe_delim Haf2 Haf3;destruct (af3 + 7)%a eqn:hsome;eauto;exfalso;solve_addr|].
+    assert (∃ wact wparams, wsstk = wact ++ wparams ∧ length wact = 7) as (wact & wparams & Hframe_eqapp & Hact_size).
+    { clear -Hframe_length. repeat (destruct wsstk;[by inversion Hframe_length|]). destruct wsstk;inversion Hframe_length.
+      exists [w;w0;w1;w2;w3;w4;w5]. eauto. }
+    rewrite Hframe_eqapp. iDestruct (region_mapsto_split _ _ b_r_adv with "Hframe") as "[Hact Hparams]";auto.
+    { clear -Ha_r_adv Hframe_delim Haf2 Haf3 Hb_r_adv. solve_addr. }
+    { rewrite /region_size Hact_size. clear -Hb_r_adv Hframe_delim Haf2 Haf3. solve_addr. }
+    iClear "Hcode". iPrologue_multi "Hprog" Hcont Hvpc link5.
+    (* reconstruct registers except r_param1 r_param2 *)
+    rewrite -!(delete_commute _ r_t4).
+    iDestruct (big_sepM_insert with "[$Hregs $Hr_t4]") as "Hregs"; [apply lookup_delete|rewrite insert_delete].
+    rewrite -!(delete_commute _ r_t3) -!delete_insert_ne//.
+    iDestruct (big_sepM_insert with "[$Hregs $Hr_t3]") as "Hregs"; [apply lookup_delete|rewrite insert_delete].
+    rewrite -!(delete_commute _ r_t2) -!delete_insert_ne//.
+    iDestruct (big_sepM_insert with "[$Hregs $Hr_t2]") as "Hregs"; [apply lookup_delete|rewrite insert_delete].
+    rewrite -!(delete_commute _ r_t1) -!delete_insert_ne//.
+    iDestruct (big_sepM_insert with "[$Hregs $Hr_t1]") as "Hregs"; [apply lookup_delete|rewrite insert_delete].
+
+    iApply (scallU_prologue_spec with "[- $HPC $Hact $Hcode $Hregs $Hr_stk]");
+      [apply Hvpc_code5| | |apply Hcont_code5|apply Hfl|auto..|apply Ha_r_adv|apply Hb_r_adv|].
+    { clear -Ha_param Haf3 Hbounds Hsize Hframe_delim Haf2. apply le_addr_withinBounds;solve_addr. }
+    { clear -Ha_param Haf3 Hbounds Hsize Hframe_delim Haf2 Hb_r_adv. apply le_addr_withinBounds;solve_addr. }
+    { repeat (apply not_elem_of_cons; split;auto). apply not_elem_of_nil. }
+    { clear. set_solver. }
+    { rewrite dom_insert_L !dom_delete_L !dom_insert_L Hdom. clear. simpl. set_solver. }
+    iSplitL "Hr_t0";[eauto|].
+    iNext. iIntros "(HPC & Hr_stk & Hr_t0 & Hregs & Hact & HscallU_prologue)".
+
+    (* TODO: fix the calling convention to take the instructions between jmp and prologue into account
+       (this can be done as a parametrised activation record, that subsegs the expected amount)? or as a parameter to prologue *)
+  Admitted. 
+
+
+
+
 
 
 
