theories/examples/world_changes.v
@@ -6,8 +6,9 @@ From cap_machine Require Export iris_extra addr_reg_sample region_macros contigu
 From cap_machine Require Import macros.
 
 (**
-   This file contains quality of life lemmas about world manipulations, for the
-   purpose of examples.
+   This file contains quality of life lemmas about world manipulations,
+   and validity in general,
+   for the purpose of examples.
  *)
 
 Section world.
@@ -21,12 +22,66 @@ Section world.
   Notation WORLD := (prodO STS_STD STS).
   Implicit Types W : WORLD.
 
+  Definition readAllowedWord (w : Word) :=
+    match w with
+    | inl _ => false
+    | inr (p,_,_,_,_) => readAllowed p
+    end.
+  Definition readAllowedUWord (w : Word) :=
+    match w with
+    | inl _ => false
+    | inr (p,_,_,_,_) => readAllowedU p
+    end.
 
-  (* For example that use a dynamic type check to reinstate validity of a revoked world *)
-  Lemma region_open_acc W W1 l p g b e a :
-    ⊢ region W1 ∗ ([∗ list] a ∈ l, (∃ p φ, ⌜forall Wv, Persistent (φ Wv)⌝ ∗ ▷ monotemp_resources W φ a p ∗ rel a p φ) ∗ ⌜(std (revoke W)) !! a = Some Revoked⌝).
+  Definition read_region (w : Word) :=
+    match w with
+    | inl _ => []
+    | inr (p,_,b,e,a) => if readAllowed p then region_addrs b e
+                        else if readAllowedU p then region_addrs b a
+                             else []
+    end.
+
+  (* If the monotonicity condition holds for some w with validity as the invariant,
+     we can infer certain bounds restrictions on that word *)
+  Lemma interp_monotonicity_bounds W a w :
+    interp W w -∗ future_pub_a_mono a interpC w -∗ ⌜(aOf w <= a)%a⌝ ∨ future_priv_mono interpC w.
+  Proof.
+    iIntros "#Hval #Hmono".
+    destruct w as [z|c].
+    { iRight. iAlways. iIntros (W1 W2 Hrelated) "#Hval' /=". rewrite !fixpoint_interp1_eq. eauto. }
+    destruct c as [ [ [ [p g] b] e] a'].
+    destruct (read_region (inr (p,g,b,e,a'))) eqn:Hlist.
+    { destruct (readAllowedU p) eqn:HraU.
+      - rewrite /read_region in Hlist.
+        assert (readAllowed p = false) as Hfalse;[destruct p;auto;inversion HraU|].
+        rewrite HraU Hfalse in Hlist. iSimpl.
+        assert (isU p = true) as HU;[destruct p;auto;inversion HraU|].
+        rewrite HU. destruct (decide (a' <= e)%a).
+    (*     iRight. iAlways. iIntros (W1 W2 Hrelated) "#Hval' /=". *)
+    (*     rewrite !fixpoint_interp1_eq. *)
+    (*     assert (region_addrs b (addr_reg.min a' e) = []) as Hnil1. *)
+    (*     { destruct (decide (addr_reg.min a' e = a'));[rewrite e0;auto|]. *)
+    (*       rewrite (region_addrs_split2 _ _ a) in Hlist. *)
+    (*       assert (addr_reg.min a' e = e) as ->;[solve_addr|]. *)
+    (*       apply region_addrs_empty. solve_addr. } *)
+    (*     assert (region_addrs (addr_reg.max b a') e = []) as Hnil2. *)
+    (*     destruct p;inversion HraU;iSimpl;auto. *)
+
+    (*     all: destruct g;simpl;try done. *)
 
 
 
+    (*   iAlways. iIntros (W1 W2 Hrelated) "#Hval' /=". *)
+    (*   simpl in Hlist. destruct (readAllowed p) eqn:Hra. *)
+    (*   - rewrite !fixpoint_interp1_eq. *)
+    (*     destruct p;inversion Hra;iSimpl;rewrite Hlist;auto. *)
+    (*     all: destruct g;simpl;done. *)
+    (*   - destruct (readAllowedU p) eqn:HraU. *)
+    (*     + rewrite !fixpoint_interp1_eq. *)
+    (*       destruct p;inversion HraU;iSimpl;auto. *)
+    (*       all: destruct g;simpl;try done. *)
+
+        (* } *)
+  Abort.
 
 End world.
