theories/rules/rules_LoadU_derived.v
@@ -24,22 +24,80 @@ Section cap_lang_rules.
     intros Hfl' Hra. destruct p'; auto. destruct p; inversion Hfl'. inversion Hra.
   Qed.
 
-  (* TODO: replace all the 1's by general z's in this file *)
 
   Lemma wb_implies_verify_access p g:
-    ∀ b e a a',
-      (a' + 1)%a = Some a ->
-      withinBounds ((p, g), b, e, a') = true ->
-      (if Addr_le_dec b a'
-       then if Addr_lt_dec a' a then if Addr_le_dec a e then Some a' else None else None
-       else None) = Some a'.
+    ∀ b e a a' zoff,
+      (zoff < 0)%Z →
+      (a' + zoff)%a = Some a →
+      withinBounds ((p, g), b, a', a) = true ->
+      (a' <= e)%a →
+      (if Addr_le_dec b a then if Addr_lt_dec a a' then if Addr_le_dec a' e then Some a else None else None else None) = Some a.
   Proof.
-    intros b e a a' Hincr Hwb.
+    intros b e a a' zoff Hlt' Hincr Hwb Hwb'.
     apply withinBounds_le_addr in Hwb as [Hle Hlt].
-    destruct (Addr_le_dec b a');[|contradiction].
-    destruct (Addr_lt_dec a' a);[|solve_addr].
-    destruct (Addr_le_dec a e);[|solve_addr].
+    destruct (Addr_le_dec b a);[|solve_addr].
+    destruct (Addr_lt_dec a a');[|solve_addr].
+    destruct (Addr_le_dec a' e);[|solve_addr].
     auto.
+  Qed.
+
+  (* loading from any offset *)
+  Lemma wp_loadU_success_any E r1 r2 zoff pc_p pc_g pc_b pc_e pc_a w w' w'' p g b e a a' pc_a'
+        pc_p' p' :
+    decodeInstrW w = LoadU r1 r2 (inl zoff) →
+    PermFlows pc_p pc_p' →
+    PermFlows p p' →
+    isCorrectPC (inr ((pc_p,pc_g),pc_b,pc_e,pc_a)) →
+    isU p = true -> (a' <= e)%a →
+    withinBounds ((p, g), b, a', a) = true →
+    (pc_a + 1)%a = Some pc_a' →
+    (a' + zoff)%a = Some a ->
+    (zoff < 0)%Z ->
+
+    {{{ ▷ PC ↦ᵣ inr ((pc_p,pc_g),pc_b,pc_e,pc_a)
+          ∗ ▷ pc_a ↦ₐ[pc_p'] w
+          ∗ ▷ r1 ↦ᵣ w''
+          ∗ ▷ r2 ↦ᵣ inr ((p,g),b,e,a')
+          ∗ ▷ a ↦ₐ[p'] w' }}}
+      Instr Executable @ E
+      {{{ RET NextIV;
+          PC ↦ᵣ inr ((pc_p,pc_g),pc_b,pc_e,pc_a')
+             ∗ r1 ↦ᵣ w'
+             ∗ pc_a ↦ₐ[pc_p'] w
+             ∗ r2 ↦ᵣ inr ((p,g),b,e,a')
+             ∗ a ↦ₐ[p'] w' }}}.
+  Proof.
+    iIntros (Hinstr Hfl Hfl' Hvpc HU Hwb Hwb2 Hpca' Hincr Hlt φ)
+            "(>HPC & >Hi & >Hr1 & >Hr2 & >Ha) Hφ".
+    pose proof (correctPC_nonO _ _ _ _ _ _ Hfl Hvpc) as Hpc_p'.
+    pose proof (isU_nonO _ _ Hfl' HU) as Hp'.
+    iDestruct (map_of_regs_3 with "HPC Hr1 Hr2") as "[Hmap (%&%&%) ]".
+    iDestruct (memMap_resource_2ne_apply with "Hi Ha") as "[Hmem %]"; auto.
+    iApply (wp_loadU with "[$Hmap $Hmem]");[apply Hinstr|apply Hpc_p'|apply Hvpc|eauto..];simplify_map_eq; eauto.
+    { by rewrite !dom_insert; set_solver+. }
+    { rewrite HU. simplify_map_eq.
+      erewrite wb_implies_verify_access;eauto.
+        by simplify_map_eq. }
+    iNext. iIntros (regs' retv) "(#Hspec & Hmem & Hmap)".
+    iDestruct "Hspec" as %Hspec.
+
+    destruct Hspec as [ | * Hfail ].
+     { (* Success *)
+       iApply "Hφ".
+       simplify_map_eq.
+       erewrite  wb_implies_verify_access in H9;eauto. simplify_eq.
+       simplify_map_eq.
+       iDestruct (memMap_resource_2ne with "Hmem") as "[Hpc_a Ha]";auto.
+       incrementPC_inv.
+       simplify_map_eq.
+       rewrite (insert_commute _ _ PC) // insert_insert insert_insert.
+       iDestruct (regs_of_map_3 with "[$Hmap]") as "[HPC [Hr1 Hr2] ]"; eauto. iFrame. }
+     { (* Failure (contradiction) *)
+       destruct Hfail; try incrementPC_inv; simplify_map_eq; eauto.
+       all: try congruence.
+       erewrite  wb_implies_verify_access in e4;eauto. simplify_eq.
+       Unshelve. all:auto.
+     }
   Qed.
 
   (* load from the top *)
@@ -68,14 +126,47 @@ Section cap_lang_rules.
   Proof.
     iIntros (Hinstr Hfl Hfl' Hvpc HU Hwb Hpca' Hincr φ)
             "(>HPC & >Hi & >Hr1 & >Hr2 & >Ha) Hφ".
+    iApply (wp_loadU_success_any with "[$Hr1 $HPC $Hr2 $Hi $Ha]");[..|iFrame];eauto.
+    - apply withinBounds_le_addr in Hwb as [Hle Hlt]. solve_addr.
+    - apply withinBounds_le_addr in Hwb as [Hle Hlt]. apply le_addr_withinBounds; solve_addr.
+    - solve_addr.
+    - lia.
+  Qed.
+
+  (* load into PC from reg *)
+  Lemma wp_loadU_success_reg_to_PC_any E r1 r2 zoff pc_p pc_g pc_b pc_e pc_a w p g b e a a1 p' g' b' e' a' a'' pc_p' p'':
+    decodeInstrW w = LoadU PC r1 (inr r2)  →
+    PermFlows pc_p pc_p' →
+    PermFlows p p'' →
+    isCorrectPC (inr ((pc_p,pc_g),pc_b,pc_e,pc_a)) →
+    isU p = true -> (a1 <= e)%a →
+    withinBounds ((p, g), b, a1, a) = true →
+    (a' + 1)%a = Some a'' →
+    (a1 + zoff)%a = Some a ->
+    (zoff < 0)%Z ->
+
+    {{{ ▷ PC ↦ᵣ inr ((pc_p,pc_g),pc_b,pc_e,pc_a)
+          ∗ ▷ pc_a ↦ₐ[pc_p'] w
+          ∗ ▷ r1 ↦ᵣ inr ((p,g),b,e,a1)
+          ∗ ▷ r2 ↦ᵣ inl zoff
+          ∗ ▷ a ↦ₐ[p''] inr ((p',g'),b',e',a') }}}
+      Instr Executable @ E
+      {{{ RET NextIV;
+          PC ↦ᵣ inr ((p',g'),b',e',a'')
+             ∗ pc_a ↦ₐ[pc_p'] w
+             ∗ r1 ↦ᵣ inr ((p,g),b,e,a1)
+             ∗ r2 ↦ᵣ inl zoff
+             ∗ a ↦ₐ[p''] inr ((p',g'),b',e',a') }}}.
+  Proof.
+    iIntros (Hinstr Hfl Hfl' Hvpc HU Hwb Hwb2 Hpca' Hincr Hlt φ)
+            "(>HPC & >Hi & >Hr1 & >Hr2 & >Ha) Hφ".
     pose proof (correctPC_nonO _ _ _ _ _ _ Hfl Hvpc) as Hpc_p'.
     pose proof (isU_nonO _ _ Hfl' HU) as Hp'.
     iDestruct (map_of_regs_3 with "HPC Hr1 Hr2") as "[Hmap (%&%&%) ]".
     iDestruct (memMap_resource_2ne_apply with "Hi Ha") as "[Hmem %]"; auto.
-    iApply (wp_loadU with "[$Hmap $Hmem]");[apply Hinstr|apply Hpc_p'|apply Hvpc|..];simplify_map_eq; eauto.
+    iApply (wp_loadU with "[$Hmap $Hmem]");[apply Hinstr |apply Hpc_p'|apply Hvpc|..];simplify_map_eq; eauto.
     { by rewrite !dom_insert; set_solver+. }
     { rewrite HU. simplify_map_eq.
-      assert ((a' + -1)%a = Some a) as ->;[solve_addr|].
       erewrite wb_implies_verify_access;eauto.
         by simplify_map_eq. }
     iNext. iIntros (regs' retv) "(#Hspec & Hmem & Hmap)".
@@ -85,19 +176,18 @@ Section cap_lang_rules.
      { (* Success *)
        iApply "Hφ".
        simplify_map_eq.
-       assert ((a0 + -1)%a = Some a) as Heq;[solve_addr|]. rewrite Heq in H9.
        erewrite  wb_implies_verify_access in H9;eauto. simplify_eq.
        simplify_map_eq.
        iDestruct (memMap_resource_2ne with "Hmem") as "[Hpc_a Ha]";auto.
        incrementPC_inv.
        simplify_map_eq.
-       rewrite (insert_commute _ _ PC) // insert_insert insert_insert.
+       rewrite insert_insert insert_insert.
        iDestruct (regs_of_map_3 with "[$Hmap]") as "[HPC [Hr1 Hr2] ]"; eauto. iFrame. }
      { (* Failure (contradiction) *)
-       destruct Hfail; try incrementPC_inv; simplify_map_eq; eauto.
-       all: try congruence.
-       assert ((a0 + -1)%a = Some a) as Heq;[solve_addr|]. rewrite Heq in e4.
-       erewrite  wb_implies_verify_access in e4;eauto. simplify_eq.
+       destruct Hfail; simplify_map_eq; first congruence.
+       all: erewrite  wb_implies_verify_access in e4;eauto.
+       * by exfalso.
+       * simplify_map_eq. eapply (incrementPC_None_inv _ _ _ _ a') in e6; last by simplify_map_eq. congruence.
        Unshelve. all:auto.
      }
   Qed.
@@ -127,40 +217,11 @@ Section cap_lang_rules.
   Proof.
     iIntros (Hinstr Hfl Hfl' Hvpc HU Hwb Hpca' Hincr φ)
             "(>HPC & >Hi & >Hr1 & >Hr2 & >Ha) Hφ".
-    pose proof (correctPC_nonO _ _ _ _ _ _ Hfl Hvpc) as Hpc_p'.
-    pose proof (isU_nonO _ _ Hfl' HU) as Hp'.
-    iDestruct (map_of_regs_3 with "HPC Hr1 Hr2") as "[Hmap (%&%&%) ]".
-    iDestruct (memMap_resource_2ne_apply with "Hi Ha") as "[Hmem %]"; auto.
-    iApply (wp_loadU with "[$Hmap $Hmem]");[apply Hinstr |apply Hpc_p'|apply Hvpc|..];simplify_map_eq; eauto.
-    { by rewrite !dom_insert; set_solver+. }
-    { rewrite HU. simplify_map_eq.
-      assert ((a1 + -1)%a = Some a) as ->;[solve_addr|].
-      erewrite wb_implies_verify_access;eauto.
-        by simplify_map_eq. }
-    iNext. iIntros (regs' retv) "(#Hspec & Hmem & Hmap)".
-    iDestruct "Hspec" as %Hspec.
-
-    destruct Hspec as [ | * Hfail ].
-     { (* Success *)
-       iApply "Hφ".
-       simplify_map_eq.
-       assert ((a0 + -1)%a = Some a) as Heq;[solve_addr|]. rewrite Heq in H9.
-       erewrite  wb_implies_verify_access in H9;eauto. simplify_eq.
-       simplify_map_eq.
-       iDestruct (memMap_resource_2ne with "Hmem") as "[Hpc_a Ha]";auto.
-       incrementPC_inv.
-       simplify_map_eq.
-       rewrite insert_insert insert_insert.
-       iDestruct (regs_of_map_3 with "[$Hmap]") as "[HPC [Hr1 Hr2] ]"; eauto. iFrame. }
-     { (* Failure (contradiction) *)
-       destruct Hfail; simplify_map_eq; first congruence.
-       all: assert ((a0 + -1)%a = Some a) as Heq;[solve_addr|]; rewrite Heq in e4;
-       erewrite  wb_implies_verify_access in e4;eauto.
-       * by exfalso.
-       * simplify_map_eq. eapply (incrementPC_None_inv _ _ _ _ a') in e6; last by simplify_map_eq. congruence.
-       Unshelve. all:auto.
-     }
+    iApply (wp_loadU_success_reg_to_PC_any with "[$Hr1 $HPC $Hr2 $Hi $Ha]");[..|iFrame];eauto.
+    - apply withinBounds_le_addr in Hwb as [Hle Hlt]. solve_addr.
+    - apply withinBounds_le_addr in Hwb as [Hle Hlt]. apply le_addr_withinBounds; solve_addr.
+    - solve_addr.
+    - lia.
   Qed.
-
 
 End cap_lang_rules.
